src/computational_monads/distribution_semantics/subsingleton.lean
@@ -1,0 +1,28 @@
+/-
+Copyright (c) 2023 Devon Tuma. All rights reserved.
+Released under Apache 2.0 license as described in the file LICENSE.
+Authors: Devon Tuma
+-/
+import computational_monads.distribution_semantics.map
+
+/-!
+# Distribution Semantics of Computations on Subsingleton Types
+
+This file gives various lemmas for probabilities of computations `oa : oracle_comp spec α`,
+when `α` is a subsingleton type, simplifying many computations.
+-/
+
+
+namespace oracle_comp
+
+open oracle_spec
+
+variables {α β γ : Type} {spec spec' : oracle_spec}
+
+/-- If a type `α` is `subsingleton` then any pair of computations are distributionally equivalent,
+so in particular they must necessarilly be just `return oa.default_result`. -/
+@[simp, simp_dist_equiv]
+lemma dist_equiv_of_subsingleton [subsingleton α] (oa : oracle_comp spec α)
+  (oa' : oracle_comp spec' α) : oa ≃ₚ oa' := subsingleton.elim _ _
+
+end oracle_comp
